WIP

theories/examples/switcher/switcher_spec.v
@@ -1,6 +1,6 @@
 From iris.algebra Require Import frac.
 From iris.proofmode Require Import proofmode.
-From cap_machine Require Import logrel interp_weakening addr_reg_sample rules proofmode.
+From cap_machine Require Import logrel fundamental interp_weakening addr_reg_sample rules proofmode.
 From cap_machine Require Import multiple_updates region_invariants_revocation.
 From cap_machine Require Import switcher.
 
@@ -87,9 +87,9 @@ Section Switcher.
     )%I.
 
   Definition switcher_inv
-    (b_switcher e_switcher a_switcher_cc : Addr)
+    (b_switcher e_switcher a_switcher_cc b_tstk e_tstk : Addr)
     (ot_switcher : OType) : iProp Σ :=
-    ∃ (b_tstk e_tstk a_tstk : Addr) (tstk_prev tstk_next : list Word),
+    ∃ (a_tstk : Addr) (tstk_prev tstk_next : list Word),
      mtdc ↦ₛᵣ WCap RWL Local b_tstk e_tstk a_tstk
      ∗ ⌜ SubBounds
          b_switcher e_switcher
@@ -315,17 +315,32 @@ Section Switcher.
   Proof.
   Admitted.
 
+Ltac focus_block' n h a_base Ha_base hi hcont :=
+  let h := constr:(h:ident) in
+  let hi := constr:(hi:ident) in
+  let hcont := constr:(hcont:ident) in
+  let x := iFresh in
+  match goal with |- context [ environments.Esnoc _ h (codefrag ?a0 _) ] =>
+    iPoseProof ((codefrag_block_acc n) with h) as (a_base) x;
+      [ once (typeclasses eauto with proofmode_focus) | ];
+    let xbase := iFresh in
+    let y := iFresh in
+    eapply coq_tactics.tac_and_destruct with x _ xbase y _ _ _;
+      [reduction.pm_reflexivity|reduction.pm_reduce;tc_solve|reduction.pm_reduce];
+    iPure xbase as Ha_base;
+    eapply coq_tactics.tac_and_destruct with y _ hi hcont _ _ _;
+      [reduction.pm_reflexivity|reduction.pm_reduce;tc_solve|reduction.pm_reduce];
+    focus_block_codefrag_facts hi a0 Ha_base
+    (* changePC_next_block a_base *)
+  end.
+Tactic Notation "focus_block'" constr(n) constr(h) "as"
+       ident(a_base) simple_intropattern(Ha_base) constr(hi) constr(hcont) :=
+  focus_block' n h a_base Ha_base hi hcont.
 
-
-  (* TODO:
-     - How to encode the number of registers to pass as arguments?
-       A possibility is to use a resource that encodes it.
-   *)
-  Lemma switcher_cc_specification
-    (E : coPset) (N : namespace)
+  Lemma switcher_ret_specification
+    (N : namespace)
     (W0 W1 : WORLD)
     (C : CmptName)
-    (g_switcher : Locality)
     (b_switcher e_switcher a_switcher_cc : Addr)
     (b_stk e_stk a_stk : Addr)
     (ot_switcher : OType)
@@ -333,6 +348,211 @@ Section Switcher.
     (w_entry_point : Sealable)
     (stk_mem : list Word)
     (arg_rmap rmap : Reg)
+    (ltemp_unknown : list Addr)
+    ( b_tstk a_tstk e_tstk a_jmp : Addr )
+    (tstk_a1 : Word)
+    (φ : val -> iPropI Σ) :
+
+    let stk_caller_save_area :=
+      [wcs0_caller;wcs1_caller;wcra_caller;wcgp_caller]
+    in
+    let callee_stk_frm_addr :=
+      finz.seq_between (a_stk ^+ 4)%a e_stk
+    in
+
+    let W0' := frame_W (std_update_multiple (revoke W0) (finz.seq_between (a_stk ^+ 4)%a e_stk) Temporary) in
+
+    let Hφ : iPropI Σ :=
+      ((∃ W2 (rmap' : Reg), ⌜related_sts_pub_world W0 W2⌝ ∗ ⌜dom rmap' = all_registers_s ∖ {[PC; cgp; cra; csp; ca0; ca1]}⌝ ∗
+                            na_own logrel_nais ⊤ ∗ sts_full_world W2 C ∗ open_region_many W2 C (finz.seq_between a_stk e_stk) ∗
+                            ([∗ list] a ∈ finz.seq_between a_stk e_stk, rel C a RWL interpC) ∗ PC ↦ᵣ updatePcPerm wcra_caller ∗ cgp ↦ᵣ wcgp_caller ∗
+                            cra ↦ᵣ wcra_caller ∗ csp ↦ᵣ WCap RWL Local b_stk e_stk a_stk ∗ (∃ warg0 : Word, ca0 ↦ᵣ warg0 ∗ interp W2 C warg0) ∗
+                            (∃ warg1 : Word, ca1 ↦ᵣ warg1 ∗ interp W2 C warg1) ∗ ([∗ map] r↦w ∈ rmap', r ↦ᵣ w ∗ ⌜w = WInt 0⌝) ∗
+                            [[a_stk,e_stk]]↦ₐ[[region_addrs_zeroes a_stk e_stk]]) -∗ WP Seq (Instr Executable) {{ v, ⌜v = HaltedV⌝ → na_own logrel_nais ⊤ }})%I
+    in
+    let htemp_unknown :=
+     ([∗ list] x ∈ ltemp_unknown, (∃ (x0 : Perm) (x1 : WORLD * CmptName * Word → iPropI Σ),
+                                    ⌜∀ Wv : WORLD * CmptName * Word, Persistent (x1 Wv)⌝ ∗ temp_resources W0 C x1 x x0 ∗
+                                    rel C x x0 x1) ∗ ⌜std (revoke W0) !! x = Some Revoked⌝)%I
+    in
+    let Pframe :=
+     (Hφ ∗ tstack_frag [tstk_a1] (finz.dist b_tstk (a_tstk ^+ 1)%a)
+      ∗ [[a_stk,(a_tstk ^+ 4)%a]]↦ₐ[[stk_caller_save_area]] ∗ htemp_unknown)%I
+    in
+    let ι := fresh_cus_name (std_update_multiple (revoke W0) callee_stk_frm_addr Temporary)
+    in
+
+    related_sts_pub_world W0' W1 ->
+    (a_switcher_cc + 79%nat)%a = Some a_jmp ->
+    (a_stk ^+ 4 < e_stk)%a ->
+    (b_stk <= a_stk)%a ->
+    (a_tstk ^+ 2 < e_tstk)%a ->
+    (b_tstk <= a_tstk)%a  ->
+    NoDup (ltemp_unknown ++ finz.seq_between a_stk e_stk) ->
+    (∀ a : finz MemNum, std W0 !! a = Some Temporary ↔ a ∈ ltemp_unknown ++ finz.seq_between a_stk e_stk) ->
+
+    ( na_inv logrel_nais N (switcher_inv b_switcher e_switcher a_switcher_cc b_tstk e_tstk ot_switcher )
+      ∗ ([∗ list] y ∈ finz.seq_between a_stk (a_stk ^+ 4)%a, rel C y RWL interpC)
+      ∗ ([∗ list] y ∈ finz.seq_between (a_stk ^+ 4)%a e_stk, rel C y RWL interpC)
+      ∗ ([∗ list] x ∈ finz.seq_between a_stk e_stk, ⌜std (revoke W0) !! x = Some Revoked⌝)
+      ∗ sts_rel_loc C ι frame_rel_pub frame_rel_pub frame_rel_priv
+      ∗ na_inv logrel_nais (nroot.@"frame") (frame_inv C ι Pframe)
+      -∗ interp W1 C (WSentry XSRW_ Local b_switcher e_switcher (a_jmp ^+ 1)%a)
+    ).
+  Proof.
+    intros stk_caller_save_area callee_stk_frm_addr W0' Hφ htemp_unknown Pframe ι
+      Ha_related_W0'_W1 Ha_jmp Hstk_ae Hstk_ba Htstk_ae Htstk_ba Hnodupl W_temps.
+    iIntros "#(Hinv_switcher & Hrel_reg_saved & Hrel_callee_frm & Htemp_opened_revoked
+              & Hsts_rel_ι & Hinv_frame)".
+
+    iEval (rewrite fixpoint_interp1_eq //=).
+    iModIntro; iIntros (rmap' W2 Hrelated_W1_W2).
+    iAssert (interp_expr interp rmap' W2 C
+               (WCap XSRW_ Local b_switcher e_switcher (a_jmp ^+ 1)%a))
+              as "Hinterp_expr" ; last iFrame "Hinterp_expr".
+
+    iIntros "([%Hfull_rmap #Hinterp_rmap] & Hrmap & Hregion & Hworld & Hna)".
+    rewrite /interp_conf /registers_pointsto.
+    iDestruct (big_sepM_delete _ _ PC with "Hrmap") as "[HPC Hrmap]"; first by rewrite lookup_insert.
+    rewrite delete_insert_delete.
+
+    (* extract register points-to *)
+    assert (exists wctp, rmap' !! ctp = Some wctp) as [wctp Hwctp].
+    { admit. }
+    iDestruct (big_sepM_delete _ _ ctp with "Hrmap") as "[Hctp Hrmap]"; first by simplify_map_eq.
+    assert (exists wcsp, rmap' !! csp = Some wcsp) as [wcsp Hwcsp].
+    { admit. }
+    iDestruct (big_sepM_delete _ _ csp with "Hrmap") as "[Hcsp Hrmap]"; first by simplify_map_eq.
+    assert (exists wcgp, rmap' !! cgp = Some wcgp) as [wcgp Hwcgp].
+    { admit. }
+    iDestruct (big_sepM_delete _ _ cgp with "Hrmap") as "[Hcgp Hrmap]"; first by simplify_map_eq.
+    assert (exists wca2, rmap' !! ca2 = Some wca2) as [wca2 Hwca2].
+    { admit. }
+    iDestruct (big_sepM_delete _ _ ca2 with "Hrmap") as "[Hca2 Hrmap]"; first by simplify_map_eq.
+    assert (exists wcs1, rmap' !! cs1 = Some wcs1) as [wcs1 Hwcs1].
+    { admit. }
+    iDestruct (big_sepM_delete _ _ cs1 with "Hrmap") as "[Hcs1 Hrmap]"; first by simplify_map_eq.
+    assert (exists wcs0, rmap' !! cs0 = Some wcs0) as [wcs0 Hwcs0].
+    { admit. }
+    iDestruct (big_sepM_delete _ _ cs0 with "Hrmap") as "[Hcs0 Hrmap]"; first by simplify_map_eq.
+    assert (exists wct0, rmap' !! ct0 = Some wct0) as [wct0 Hwct0].
+    { admit. }
+    iDestruct (big_sepM_delete _ _ ct0 with "Hrmap") as "[Hct0 Hrmap]"; first by simplify_map_eq.
+    assert (exists wct1, rmap' !! ct1 = Some wct1) as [wct1 Hwct1].
+    { admit. }
+    iDestruct (big_sepM_delete _ _ ct1 with "Hrmap") as "[Hct1 Hrmap]"; first by simplify_map_eq.
+
+    (* open switcher invariant *)
+    iMod (na_inv_acc with "Hinv_switcher Hna")
+      as "(Hswitcher_inv & Hna & Hclose_switcher_inv)" ; auto.
+    rewrite /switcher_inv.
+    iDestruct "Hswitcher_inv"
+      as (a_tstk' tstk_prev' tstk_next')
+           "(>Hmtdc & >%Hbounds & >Hcode & >Hb_switcher & >Htstk_prev & >Htstk & Hstack_full & Hstack_frag_next & #Hp_ot_switcher)".
+    codefrag_facts "Hcode".
+    rename H into Hcont_switcher_region; clear H0.
+    iHide "Hclose_switcher_inv" as hclose_switcher_inv.
+    iHide "Hinv_switcher" as hinv_switcher.
+
+    (* open frame invariant *)
+    iMod (na_inv_acc with "Hinv_frame Hna")
+      as "(Hframe & Hna & Hclose_frame_inv)" ; auto.
+    { admit. }
+    iEval (rewrite /frame_inv) in "Hframe".
+    iDestruct "Hframe" as (x) "[Hsts_state_frame Hframe]".
+
+
+
+    (* focus_block 6 "Hcode" as a_jmp' Ha_jmp' "Hcode" "Hcont"; iHide "Hcont" as hcont. *)
+    (* rewrite /switcher_instrs. *)
+    focus_block_0 "Hcode" as "Hcode" "Hcont"; iHide "Hcont" as hcont.
+    unfocus_block "Hcode" "Hcont" as "Hcode"; subst hcont.
+    focus_block' 5 "Hcode" as a5 Ha5 "Hcode" "Hcont"; iHide "Hcont" as hcont.
+    assert (a5 = a_jmp) by solve_addr ; simplify_eq.
+
+
+    (* ReadSR ctp mtdc *)
+    iInstr "Hcode".
+    { done. }
+
+    (* TODO extract as lemma about frame_W *)
+    iDestruct (sts_full_state_loc with "[$] [$]") as "%Hx".
+    iDestruct (sts_full_rel_loc with "[$] [$]") as "%Hxrel".
+    assert (x = true) as ->.
+    {
+      assert (W0'.2.1 !! ι = Some (encode true)) by (by rewrite /W0' /frame_W /ι lookup_insert).
+      assert (W0'.2.2 !! ι = Some ( convert_rel frame_rel_pub, convert_rel frame_rel_pub, convert_rel frame_rel_priv))
+        by (by rewrite /W0' /frame_W /ι lookup_insert).
+      assert (related_sts_pub_world W0' W2) as Hrelated by (eapply related_sts_pub_trans_world; eauto).
+
+      destruct Hrelated as [ _ [_ [_ Hrelated ] ] ].
+      specialize (Hrelated ι _ _ _ _ _ _ H2 Hxrel).
+      destruct Hrelated as (_ & _ & _ & Hrelated).
+      specialize (Hrelated _ _ H1 Hx).
+      rewrite /convert_rel /frame_rel_pub /= in Hrelated.
+      apply rtc_inv in Hrelated.
+      destruct Hrelated.
+      + by inv H3.
+      + destruct H3 as (? & (? & ? & Hcontra) & _).
+        naive_solver.
+    }
+
+    iDestruct "Hframe" as "(Hφ & Hstack_frag & tstk & Htemp_unknown)".
+    assert (a_tstk' = (a_tstk^+1)%a ) as ->.
+    { (* TODO I should be able to derive this information from the tstack resources, somehow *) admit. }
+    replace (finz.dist b_tstk ((a_tstk ^+ 1) ^+ 1)%a) with ((finz.dist b_tstk (a_tstk ^+ 1)%a) + 1).
+    2:{ admit. }
+
+    iCombine "Hstack_frag Hstack_frag_next" as "Hstack_frag".
+    rewrite -tstack_frag_combine_cons.
+    iDestruct (tstack_agree with "[$] [$Hstack_frag]") as "%Htstack_cur".
+    destruct (Htstack_cur) as (l0' & l1' & Hlen_l0' & Htstks1').
+    assert ( l1' = [] ∧ tstk_prev' = l0'++[tstk_a1] ) as [-> ->].
+    { admit. }
+    rewrite (region_pointsto_split _ _ (a_tstk ^+ 1)%a); [ | solve_addr | auto].
+    iDestruct "Htstk_prev" as "[Htstk_prev Htstk_cur]".
+    iDestruct (region_pointsto_single with "Htstk_cur") as (v) "[Htstk_cur ->]"; first solve_addr.
+
+
+    (* Load csp ctp *)
+    iInstr "Hcode".
+    { admit. }
+
+    (* Lea ctp (-1)%Z *)
+    (* WriteSR mtdc ctp *)
+    (* Load cgp csp *)
+    (* Lea csp (-1)%Z *)
+    (* Load ca2 csp *)
+    (* Lea csp (-1)%Z *)
+    (* Load cs1 csp *)
+    (* Lea csp (-1)%Z *)
+    (* Load cs0 csp *)
+    (* GetE ct0 csp *)
+    (* GetA ct1 csp *)
+    (* iInstr "Hcode". *)
+
+
+
+
+  Admitted.
+
+
+  (* TODO:
+     - How to encode the number of registers to pass as arguments?
+       A possibility is to use a resource that encodes it.
+   *)
+  Lemma switcher_cc_specification
+    (N : namespace)
+    (W0 W1 : WORLD)
+    (C : CmptName)
+    (b_switcher e_switcher a_switcher_cc : Addr)
+    (b_stk e_stk a_stk : Addr)
+    (ot_switcher : OType)
+    (wcgp_caller wcra_caller wcs0_caller wcs1_caller : Word)
+    (w_entry_point : Sealable)
+    (stk_mem : list Word)
+    (arg_rmap rmap : Reg)
+    (b_tstk e_tstk : Addr)
     (φ : val -> iPropI Σ) :
 
     (* ct1 must contain the target entry points, which needs to be sealed with ot_switcher *)
@@ -353,14 +573,13 @@ Section Switcher.
 
     is_arg_rmap arg_rmap ->
     dom rmap = all_registers_s ∖ ((dom arg_rmap) ∪ {[ PC ; cgp ; cra ; csp ; cs0 ; cs1 ; ct1 ]} ) ->
-    ↑N ⊆ E →
 
-    ( na_inv logrel_nais N (switcher_inv b_switcher e_switcher a_switcher_cc ot_switcher)
+    ( na_inv logrel_nais N (switcher_inv b_switcher e_switcher a_switcher_cc b_tstk e_tstk ot_switcher )
 
       (* PRE-CONDITION *)
-      ∗ na_own logrel_nais E
+      ∗ na_own logrel_nais ⊤
       (* Registers *)
-      ∗ PC ↦ᵣ WCap XSRW_ g_switcher b_switcher e_switcher a_switcher_cc
+      ∗ PC ↦ᵣ WCap XSRW_ Local b_switcher e_switcher a_switcher_cc
       ∗ cgp ↦ᵣ wcgp_caller
       ∗ cra ↦ᵣ wcra_caller
       (* Stack register *)
@@ -396,7 +615,7 @@ Section Switcher.
                 (* We receive a public future world of the world pre switcher call *)
                 ⌜ related_sts_pub_world W0 W2 ⌝
                 ∗ ⌜ dom rmap' = all_registers_s ∖ {[ PC ; cgp ; cra ; csp ; ca0 ; ca1 ]} ⌝
-                ∗ na_own logrel_nais E
+                ∗ na_own logrel_nais ⊤
                 (* Interpretation of the world *)
                 ∗ sts_full_world W2 C
                 ∗ open_region_many W2 C (finz.seq_between a_stk e_stk)
@@ -410,13 +629,13 @@ Section Switcher.
                 ∗ (∃ warg1, ca1 ↦ᵣ warg1 ∗ interp W2 C warg1)
                 ∗ ( [∗ map] r↦w ∈ rmap', r ↦ᵣ w ∗ ⌜ w = WInt 0 ⌝ )
                 ∗ [[ a_stk , e_stk ]] ↦ₐ [[ region_addrs_zeroes a_stk e_stk ]])
-            -∗ WP Seq (Instr Executable) {{ λ v, φ v ∨ ⌜v = FailedV⌝ }}
-          )
+            -∗ WP Seq (Instr Executable) {{ v, ⌜v = HaltedV⌝ → na_own logrel_nais ⊤ }})
     )
-    ⊢ (WP Seq (Instr Executable) {{ λ v, φ v ∨ ⌜v = FailedV⌝ }})%I.
+    ⊢ WP Seq (Instr Executable)
+       {{ v, ⌜v = HaltedV⌝ → na_own logrel_nais ⊤ }}.
   Proof.
     intros Hwct1_caller Hstk_caller_save_area Hstk_caller_frm_pre Hstk_pre_jmp W0'
-      Harg_map Hrmap HNE.
+      Harg_map Hrmap.
     iIntros "(#Hinv_switcher & Hna & HPC & Hcgp & Hcra & Hcsp & Hct1 & #Hinterp_ct1 & Hcs0 & Hcs1
                 & Hargmap & Hrmap & Hstk & Hworld & Hregion & Hstd_stk & %Hrelated_W1
                 & Hnext_world & Hφ)".
@@ -432,7 +651,7 @@ Section Switcher.
       as "(Hswitcher_inv & Hna & Hclose_switcher_inv)" ; auto.
     rewrite /switcher_inv.
     iDestruct "Hswitcher_inv"
-      as (b_tstk e_tstk a_tstk tstk_prev tstk_next)
+      as (a_tstk tstk_prev tstk_next)
            "(>Hmtdc & >%Hbounds & >Hcode & >Hb_switcher & >Htstk_prev & >Htstk & Hstack_full & Hstack_frag_next & #Hp_ot_switcher)".
     codefrag_facts "Hcode".
     rename H into Hcont_switcher_region; clear H0.
@@ -722,8 +941,6 @@ Section Switcher.
     { apply withinBounds_true_iff; solve_addr. (* TODO solve_pure *) }
     rewrite Heq_entry_point.
 
-
-
     (* Load cs0 ct1 *)
     iDestruct (region_open_perm with "[$Hrel_atbl $Hregion $Hworld]")
       as (watbl) "(Hregion & Hworld & Hstd_atbl & Ha_tbl & _ & HmonoReq_atbl & #HPatbl)"
@@ -773,6 +990,9 @@ Section Switcher.
                 with "[$Hregion $Hstd_btbl $Ha_tbl $HmonoReq_btbl $Hrel_btbl]")
                 as "Hregion"; eauto.
     { iSplit; auto. iNext; eauto. }
+
+    iEval (cbn) in "Hinterp_wbtbl".
+    iDestruct (interp_updatePcPerm with "Hinterp_wbtbl") as "Hjmp_callee_pc".
 
     (* Lea ct1 1%Z *)
     iInstr "Hcode".
@@ -907,16 +1127,18 @@ Section Switcher.
 
     (* allocate frame invariant *)
     rewrite tstack_frag_combine_cons.
+    iHide "Htemp_unknown" as htemp_unknown.
     iDestruct "Hstack_frag_next" as "[Hstack_frag_current Hstack_frag_next]".
     set (Pframe := (hφ0
                     ∗ tstack_frag [tstk_a1] (finz.dist b_stk (a_tstk ^+ 1)%a)
                     ∗ [[a_stk,(a_tstk ^+ 4)%a]]↦ₐ[[Hstk_caller_save_area]]
+                    ∗ htemp_unknown
                    )%I).
     iMod (na_inv_alloc
             logrel_nais
             ⊤ (nroot .@ "frame")
             (frame_inv C ι Pframe)
-           with "[$Hsts_loc_ι Hφ Hstack_frag_current Ha1_stk Ha2_stk Ha3_stk Ha4_stk ]") as "#Hinv_frame".
+           with "[$Hsts_loc_ι $Hφ $Htemp_unknown Hstack_frag_current Ha1_stk Ha2_stk Ha3_stk Ha4_stk ]") as "#Hinv_frame".
     { iNext; iFrame.
       rewrite /Hstk_caller_save_area.
       admit.
@@ -928,6 +1150,7 @@ Section Switcher.
     (* close switcher invariant *)
     iMod ("Hclose_switcher_inv" with
            "[$Hna Hmtdc Hcode Hb_switcher Htstk_prev Ha1_tstk Htstk Hstack_full Hstack_frag_next]")
+      as "Hna"
     .
     { iNext; iFrame "Hmtdc Hstack_full".
       iSplit; first done.
@@ -942,17 +1165,196 @@ Section Switcher.
       admit.
     }
 
-    iAssert (interp W1 C (WSentry XSRW_ g_switcher b_switcher e_switcher (a_jmp ^+ 1)%a)) as "Hinterp_return".
+    iAssert (interp W1 C (WSentry XSRW_ Local b_switcher e_switcher (a_jmp ^+ 1)%a)) as "Hinterp_return".
     { shelve. }
 
+    iCombine "Harg_rmap' Hrmap'" as "Hrmap'".
+    rewrite -(big_sepM_union _ arg_rmap' rmap').
+    2: {
+      clear -Harg_rmap' Hrmap'.
+      rewrite /is_arg_rmap in Harg_rmap'; simplify_eq.
+      apply map_disjoint_dom.
+      set_solver.
+    }
+    iDestruct (big_sepM_insert _ _ cgp with "[$Hrmap' $Hcgp $Hinterp_wbtbl1]") as "Hrmap'".
+    {
+      clear -Harg_rmap' Hrmap'.
+      rewrite /is_arg_rmap in Harg_rmap'; simplify_eq.
+      rewrite /dom_arg_rmap in Hrmap'.
+      apply not_elem_of_dom.
+      set_solver.
+    }
+    iDestruct (big_sepM_insert _ _ cra with "[$Hrmap' $Hcra $Hinterp_return]") as "Hrmap'".
+    {
+      clear -Harg_rmap' Hrmap'.
+      rewrite /is_arg_rmap in Harg_rmap'; simplify_eq.
+      rewrite /dom_arg_rmap in Hrmap'.
+      apply not_elem_of_dom.
+      set_solver.
+    }
+    iDestruct (big_sepM_insert _ _ csp with "[$Hrmap' $Hcsp $Hinterp_csp]") as "Hrmap'".
+    {
+      clear -Harg_rmap' Hrmap'.
+      rewrite /is_arg_rmap in Harg_rmap'; simplify_eq.
+      rewrite /dom_arg_rmap in Hrmap'.
+      do 2 rewrite lookup_insert_ne //.
+      apply not_elem_of_dom.
+      set_solver.
+    }
+    iDestruct (big_sepM_insert _ _ PC with "[$Hrmap' $HPC $Hinterp_wbtbl]") as "Hrmap'".
+    {
+      clear -Harg_rmap' Hrmap'.
+      rewrite /is_arg_rmap in Harg_rmap'; simplify_eq.
+      rewrite /dom_arg_rmap in Hrmap'.
+      do 3 rewrite lookup_insert_ne //.
+      apply not_elem_of_dom.
+      set_solver.
+    }
 
+    match goal with
+    | _ : _ |- context [<[PC:=?w]> ?m] =>
+        set (rmap'' := <[PC:=w]> m)
+    end.
+    rewrite -(insert_id rmap'' PC (WCap RX Global bpcc epcc apcc)).
+    2: { by subst rmap'' ; rewrite lookup_insert. }
+    iEval (rewrite big_sepM_sep) in "Hrmap'".
+    iDestruct "Hrmap'" as "[Hrmap_mapsto Hrmap_interp]".
+    iApply "Hjmp_callee_pc"; iFrame.
+    rewrite /interp_reg //=.
+
+    iSplitR "Hrmap_interp".
+    + clear -Hrmap' Harg_rmap'.
+      subst hinv_switcher hφ0 htemp_unknown Pframe rmap''.
+      iPureIntro.
+      intros r; cbn.
+      destruct (decide (r = PC)) as [Hrpc | Hrpc]; simplify_eq; first by rewrite lookup_insert.
+      rewrite lookup_insert_ne //.
+      destruct (decide (r = csp)) as [Hrcsp | Hrcsp]; simplify_eq; first by rewrite lookup_insert.
+      rewrite lookup_insert_ne //.
+      destruct (decide (r = cra)) as [Hrcra | Hrcra]; simplify_eq; first by rewrite lookup_insert.
+      rewrite lookup_insert_ne //.
+      destruct (decide (r = cgp)) as [Hrcgp | Hrcgp]; simplify_eq; first by rewrite lookup_insert.
+      rewrite lookup_insert_ne //.
+      apply elem_of_dom.
+      rewrite dom_union.
+      rewrite elem_of_union.
+      destruct (decide (r ∈ dom arg_rmap')); first by left.
+      right.
+      rewrite Harg_rmap' in n.
+      assert (r ∉ ({[PC; cra; cgp; csp]} : gset RegName)).
+      { set_solver.  }
+      rewrite Hrmap'.
+      rewrite elem_of_difference.
+      split; first by apply all_registers_s_correct.
+      set_solver.
+    + iIntros (r w HrPC Hr).
+      subst rmap''.
+      admit. (* easy, just boring stuff *)
+
+
+
+    (* Proof of the return *)
+    Unshelve.
     (* TODO that's the interesting part !!!!
       - show that rmap' is safe to share
       - show that cra is safe to share
      *)
 
+    iClear
+      "Hp_ot_switcher HmonoReq Hseal_pred_Pct1 Hrel_btbl Hrel_btbl1 Hrel_atbl
+      HPct1_borrow Hjmp_callee_pc Hinterp_wbtbl1 Hinterp_csp Hinterp_wbtbl".
+    clear
+      (* Ha_jmp a_jmp *)
+      Hrmap' Harg_rmap'
+      Ha_clear_pre_reg2 a_clear_pre_reg2
+      Ha_clear_pre_reg1 a_clear_pre_reg1
+      H1 Ha_unseal a_unseal
+      Ha_clear_stk1 a_clear_stk1.
+    clear Hwctp Hwct2 Hrmap rmap rmap'.
+    subst hclose_switcher_inv hφ.
+    clear Hstk_pre_jmp.
+    cbn in Ha_jmp.
+    clear Harg_map.
+    clear Hnargs arg_rmap' nargs off_entry Hot_switcher Hstd_atbl Hstd_btbl1 Hstd_btbl Ha_tbl_in i_a_tbl.
+    clear Hatbl Hbtbl Hbtbl1.
+    clear wct2 wctp stk_wa stk_wa1 stk_wa2 stk_wa3 stk_mem' tstk_next'.
+
+  iApply switcher_cc_specification; eauto.
+  iFrame "#".
 
   Admitted.
+
+
+
+    (WSentry XSRW_ Local b_switcher e_switcher (a_jmp ^+ 1)%a)n
+
+
+
+
+    (
+
+      (* PRE-CONDITION *)
+      ∗ na_own logrel_nais ⊤
+      (* Registers *)
+      ∗ PC ↦ᵣ WCap XSRW_ Local b_switcher e_switcher a_switcher_cc
+      ∗ cgp ↦ᵣ wcgp_caller
+      ∗ cra ↦ᵣ wcra_caller
+      (* Stack register *)
+      ∗ csp ↦ᵣ WCap RWL Local b_stk e_stk a_stk
+      (* Entry point of the target compartment *)
+      ∗ ct1 ↦ᵣ wct1_caller ∗ interp W1 C wct1_caller
+      ∗ cs0 ↦ᵣ wcs0_caller
+      ∗ cs1 ↦ᵣ wcs1_caller
+      (* Argument registers, need to be safe-to-share *)
+      ∗ ( [∗ map] rarg↦warg ∈ arg_rmap, rarg ↦ᵣ warg ∗ interp W1 C warg (* ∗ ⌜ isWLword warg ⌝ *) )
+      (* All the other registers *)
+      ∗ ( [∗ map] r↦w ∈ rmap, r ↦ᵣ w )
+
+      (* Stack frame *)
+      ∗ [[ a_stk , e_stk ]] ↦ₐ [[ stk_mem ]]
+
+      (* Interpretation of the world, at the moment of the switcher_call *)
+      ∗ sts_full_world W0 C
+      ∗ open_region_many W0 C (finz.seq_between a_stk e_stk)
+      ∗ ([∗ list] a ∈ (finz.seq_between a_stk e_stk), rel C a RWL interpC ∗ sts_state_std C a Temporary)
+      (* ∗ (⌜ forall a, a ∈ (finz.seq_between a_stk e_stk) -> (std W0) !! a = Some Temporary ⌝) *)
+        (* region W0 C *)
+      ∗ (⌜ related_sts_pub_world W0' W1 ⌝)
+
+      (* Transformation of the world, before the jump to the adversary *)
+      ∗ ( region W0' C ∗ sts_full_world W0' C
+          ==∗
+          region W1 C ∗ sts_full_world W1 C)
+
+
+      (* POST-CONDITION *)
+      ∗ ▷ ( (∃ (W2 : WORLD) (rmap' : Reg),
+                (* We receive a public future world of the world pre switcher call *)
+                ⌜ related_sts_pub_world W0 W2 ⌝
+                ∗ ⌜ dom rmap' = all_registers_s ∖ {[ PC ; cgp ; cra ; csp ; ca0 ; ca1 ]} ⌝
+                ∗ na_own logrel_nais ⊤
+                (* Interpretation of the world *)
+                ∗ sts_full_world W2 C
+                ∗ open_region_many W2 C (finz.seq_between a_stk e_stk)
+                ∗ ([∗ list] a ∈ (finz.seq_between a_stk e_stk), rel C a RWL interpC )
+                (* ∗  *)
+                ∗ PC ↦ᵣ updatePcPerm wcra_caller
+                (* cgp is restored, cra points to the next  *)
+                ∗ cgp ↦ᵣ wcgp_caller ∗ cra ↦ᵣ wcra_caller
+                ∗ csp ↦ᵣ WCap RWL Local b_stk e_stk a_stk
+                ∗ (∃ warg0, ca0 ↦ᵣ warg0 ∗ interp W2 C warg0)
+                ∗ (∃ warg1, ca1 ↦ᵣ warg1 ∗ interp W2 C warg1)
+                ∗ ( [∗ map] r↦w ∈ rmap', r ↦ᵣ w ∗ ⌜ w = WInt 0 ⌝ )
+                ∗ [[ a_stk , e_stk ]] ↦ₐ [[ region_addrs_zeroes a_stk e_stk ]])
+            -∗ WP Seq (Instr Executable) {{ v, ⌜v = HaltedV⌝ → na_own logrel_nais ⊤ }})
+    )
+    ⊢ WP Seq (Instr Executable)
+       {{ v, ⌜v = HaltedV⌝ → na_own logrel_nais ⊤ }}.
+  Proof.
+  Lemma switcher_return :
+
+  
+
 
   Lemma switcher_interp (W : WORLD) (C : CmptName) (N : namespace)
     (b_switcher e_switcher a_switcher_cc : Addr) (ot_switcher : OType) :
